Cslib/Computability/CombinatoryLogic/NormalOrder.lean
@@ -1,0 +1,58 @@
+import Cslib.Computability.CombinatoryLogic.Evaluation
+import Mathlib.Data.List.Induction
+
+namespace SKI
+
+inductive Prim where
+  | S₀ | K₀ | I₀
+
+@[coe]
+def Prim.toSKI : Prim → SKI
+  | S₀ => S
+  | K₀ => K
+  | I₀ => I
+
+open Prim
+
+instance PrimToSKI : Coe Prim SKI := ⟨Prim.toSKI⟩
+
+protected structure Tree where
+  head : Prim
+  tail : List SKI.Tree
+
+def Tree.toSKI : SKI.Tree → SKI
+  | ⟨x, xs⟩ => (↑x : SKI).applyList <| List.map Tree.toSKI xs
+
+protected def toTree : SKI → SKI.Tree
+  | S => ⟨S₀, []⟩
+  | K => ⟨K₀, []⟩
+  | I => ⟨I₀, []⟩
+  | a ⬝ b => let ⟨x,xs⟩ := a.toTree; ⟨x, xs ++ [b.toTree]⟩
+
+def Tree.size : SKI.Tree → Nat
+  | ⟨x, xs⟩ => 1 + (List.sum <| List.map Tree.size xs)
+
+lemma coe_toTree (x : Prim) : (↑x : SKI).toTree = ⟨x, []⟩ := by cases x <;> rfl
+
+theorem toTree_of_toSKI (t : SKI.Tree) : t.toSKI.toTree = t := by
+  let ⟨x,xs⟩ := t
+  refine List.reverseRecOn xs ?nil ?app
+  case nil => simp [Tree.toSKI, applyList, coe_toTree]
+  case app =>
+    intro ys y ih
+    -- have : Tree.size y < Tree.size ⟨x, xs⟩ := by sorry
+    simp only [Tree.toSKI, List.map_append, List.map_cons, List.map_nil, applyList_concat]
+    have : (↑x : SKI).applyList (List.map Tree.toSKI ys) = (⟨x, ys⟩ : SKI.Tree).toSKI := by
+      simp [Tree.toSKI]
+    simp! [this, ih, toTree_of_toSKI y]
+  termination_by Tree.size t
+  decreasing_by sorry
+
+
+
+-- def treeEquiv : Equiv SKI SKI.Tree where
+--   toFun := SKI.toTree
+--   invFun := SKI.Tree.toSKI
+
+--   left_inv := by
+--     intro x
